Add post condition to vale wrapper

vale/code/arch/x64/interop/GCMencryptOpt_stdcalls.fst
@@ -9,6 +9,8 @@ open GCM_helpers
 open FStar.Calc
 open FStar.Int.Cast
 open FStar.Integers
+open Arch.Types
+open Workarounds
 
 #set-options "--z3rlimit 400 --max_fuel 0 --max_ifuel 0"
 
@@ -130,81 +132,66 @@ val gcm128_encrypt_opt':
       length_aux5 hkeys_b;
       low_buffer_read TUInt8 TUInt128 h0 hkeys_b 0 == aes_encrypt_LE AES_128 (Ghost.reveal key) (Mkfour 0 0 0 0))
     )
-    (ensures fun h0 _ h1 -> True)
-    //   B.modifies (B.loc_union (B.loc_buffer tag_b)
-    //               (B.loc_union (B.loc_buffer iv_b)
-    //               (B.loc_union (B.loc_buffer scratch_b)
-    //               (B.loc_union (B.loc_buffer out128x6_b)
-    //               (B.loc_union (B.loc_buffer out128_b)
-    //               (B.loc_buffer inout_b)))))) h0 h1 /\
-    //   (8 * (UInt64.v plain_num) < pow2_32 /\
-    //    8 * (UInt64.v auth_bytes) < pow2_32 /\ (
-    //    let in128x6_d = get_downview in128x6_b in
-    //    length_aux3 in128x6_b (UInt64.v len128x6);
-    //    let in128x6_u = UV.mk_buffer in128x6_d Views.up_view128 in
-    //    let in128_d = get_downview in128_b in
-    //    length_aux3 in128_b (UInt64.v len128_num);
-    //    let in128_u = UV.mk_buffer in128_d Views.up_view128 in
-    //    let inout_d = get_downview inout_b in
-    //    length_aux3 inout_b 1;      
-    //    let inout_u = UV.mk_buffer inout_d Views.up_view128 in       
-    //    let out128x6_d = get_downview out128x6_b in
-    //    length_aux3 out128x6_b (UInt64.v len128x6);
-    //    let out128x6_u = UV.mk_buffer out128x6_d Views.up_view128 in
-    //    let out128_d = get_downview out128_b in
-    //    length_aux3 out128_b (UInt64.v len128_num);
-    //    let out128_u = UV.mk_buffer out128_d Views.up_view128 in       
-    //    length_aux4 iv_b;
-    //    DV.length_eq (get_downview iv_b);
-    //    let iv_LE = low_buffer_read TUInt8 TUInt128 h0 iv_b 0 in
-    //    let iv_BE = reverse_bytes_quad32 iv_LE in
-    //    let ctr_BE_1 = Mkfour 1 iv_BE.lo1 iv_BE.hi2 iv_BE.hi3 in
-    //    let ctr_BE_2 = Mkfour 2 iv_BE.lo1 iv_BE.hi2 iv_BE.hi3 in
-    //    let plain_in =
-    //      if (UInt64.v plain_num > (UInt64.v len128x6 + UInt64.v len128_num) * 128/8) then
-    //        Seq.append (Seq.append (UV.as_seq h0 in128x6_u) (UV.as_seq h0 in128_u))
-    //                   (UV.as_seq h0 inout_u)
-    //      else Seq.append (UV.as_seq h0 in128x6_u) (UV.as_seq h0 in128_u)
-    //    in let cipher_out =
-    //      if (UInt64.v plain_num > (UInt64.v len128x6 + UInt64.v len128_num) * 128/8) then
-    //        Seq.append (Seq.append (UV.as_seq h1 out128x6_u) (UV.as_seq h1 out128_u))
-    //                   (UV.as_seq h1 inout_u)
-    //      else Seq.append (UV.as_seq h1 out128x6_u) (UV.as_seq h1 out128_u)
-    //    in gctr_partial AES_128 (UInt64.v len128x6 + UInt64.v len128_num + 1) plain_in cipher_out (Ghost.reveal key) ctr_BE_2 /\ (
-    //    DV.length_eq (get_downview hkeys_b);
-    //    let h = reverse_bytes_quad32 (low_buffer_read TUInt8 TUInt128 h1 hkeys_b 0) in
-    //    let length_quad = reverse_bytes_quad32 (Mkfour (8 * UInt64.v plain_num) 0 (8 * UInt64.v auth_bytes) 0) in
-    //    let auth_d = get_downview auth_b in
-    //    length_aux3 auth_b (UInt64.v auth_num);
-    //    let auth_u = UV.mk_buffer auth_d Views.up_view128 in
-    //    let abytes_d = get_downview abytes_b in
-    //    length_aux3 abytes_b 1;      
-    //    let abytes_u = UV.mk_buffer abytes_d Views.up_view128 in        
-    //    let cipher_bytes =
-    //      if UInt64.v plain_num > (UInt64.v len128x6 + UInt64.v len128_num) * 128/8 then
-    //        UV.as_seq h1 inout_u
-    //      else Seq.empty
-    //    in let auth_in =
-    //      if UInt64.v auth_bytes > UInt64.v auth_num * 128 / 8 then
-    //        Seq.append (Seq.append (Seq.append (Seq.append (Seq.append
-    //          (UV.as_seq h0 auth_u) (UV.as_seq h0 abytes_u))
-    //          (UV.as_seq h1 out128x6_u))
-    //          (UV.as_seq h1 out128_u))
-    //          cipher_bytes)
-    //          (Seq.create 1 length_quad)
-    //      else
-    //        Seq.append (Seq.append (Seq.append (Seq.append
-    //          (UV.as_seq h0 auth_u) (UV.as_seq h1 out128x6_u))
-    //          (UV.as_seq h1 out128_u))
-    //          cipher_bytes)
-    //          (Seq.create 1 length_quad)
-    //    in
-    //    DV.length_eq (get_downview tag_b);
-    //    low_buffer_read TUInt8 TUInt128 h1 tag_b 0 ==
-    //      gctr_encrypt_block ctr_BE_1 (ghash_LE h auth_in) AES_128 (Ghost.reveal key) 0
-    //      )
-    //      ))
-    // )
+    (ensures fun h0 _ h1 ->
+      B.modifies (B.loc_union (B.loc_buffer tag_b)
+                  (B.loc_union (B.loc_buffer iv_b)
+                  (B.loc_union (B.loc_buffer scratch_b)
+                  (B.loc_union (B.loc_buffer out128x6_b)
+                  (B.loc_union (B.loc_buffer out128_b)
+                  (B.loc_buffer inout_b)))))) h0 h1 /\
+      (8 * (UInt64.v plain_num) < pow2_32 /\
+       8 * (UInt64.v auth_bytes) < pow2_32 /\ (
+       let in128x6_d = get_downview in128x6_b in
+       length_aux3 in128x6_b (UInt64.v len128x6);
+       let in128x6_u = UV.mk_buffer in128x6_d Views.up_view128 in
+       let in128_d = get_downview in128_b in
+       length_aux3 in128_b (UInt64.v len128_num);
+       let in128_u = UV.mk_buffer in128_d Views.up_view128 in
+       let inout_d = get_downview inout_b in
+       length_aux3 inout_b 1;      
+       let inout_u = UV.mk_buffer inout_d Views.up_view128 in       
+       let out128x6_d = get_downview out128x6_b in
+       length_aux3 out128x6_b (UInt64.v len128x6);
+       let out128x6_u = UV.mk_buffer out128x6_d Views.up_view128 in
+       let out128_d = get_downview out128_b in
+       length_aux3 out128_b (UInt64.v len128_num);
+       let out128_u = UV.mk_buffer out128_d Views.up_view128 in       
+       length_aux4 iv_b;
+       DV.length_eq (get_downview iv_b);
+       let iv_LE = low_buffer_read TUInt8 TUInt128 h0 iv_b 0 in
+       let iv = be_quad32_to_bytes (reverse_bytes_quad32 iv_LE) in
+       let plain_in =
+         if (UInt64.v plain_num > (UInt64.v len128x6 + UInt64.v len128_num) * 128/8) then
+           Seq.append (Seq.append (UV.as_seq h0 in128x6_u) (UV.as_seq h0 in128_u))
+                      (UV.as_seq h0 inout_u)
+         else Seq.append (UV.as_seq h0 in128x6_u) (UV.as_seq h0 in128_u)
+       in let plain_bytes = slice_work_around (le_seq_quad32_to_bytes plain_in) (UInt64.v plain_num)
+       in let cipher_out =
+         if (UInt64.v plain_num > (UInt64.v len128x6 + UInt64.v len128_num) * 128/8) then
+           Seq.append (Seq.append (UV.as_seq h1 out128x6_u) (UV.as_seq h1 out128_u))
+                      (UV.as_seq h1 inout_u)
+         else Seq.append (UV.as_seq h1 out128x6_u) (UV.as_seq h1 out128_u)
+       in let cipher_bytes = slice_work_around (le_seq_quad32_to_bytes cipher_out) (UInt64.v plain_num)
+       in let auth_d = get_downview auth_b in
+       length_aux3 auth_b (UInt64.v auth_num);
+       let auth_u = UV.mk_buffer auth_d Views.up_view128 in
+       let abytes_d = get_downview abytes_b in
+       length_aux3 abytes_b 1;      
+       let abytes_u = UV.mk_buffer abytes_d Views.up_view128 in        
+       let auth_in =
+         if UInt64.v auth_bytes > UInt64.v auth_num * 128 / 8 then
+           Seq.append (UV.as_seq h0 auth_u) (UV.as_seq h0 abytes_u)
+         else UV.as_seq h0 auth_u
+       in
+      let auth_bytes = slice_work_around (le_seq_quad32_to_bytes auth_in) (UInt64.v auth_bytes) in
+      4096 * (Seq.length plain_bytes) < pow2_32 /\
+      4096 * (Seq.length auth_bytes) < pow2_32 /\
+      (let cipher, tag = gcm_encrypt_LE AES_128 (seq_nat32_to_seq_nat8_LE (Ghost.reveal key)) iv plain_bytes auth_bytes in
+      Seq.equal cipher cipher_bytes /\
+      (DV.length_eq (get_downview tag_b);
+      le_quad32_to_bytes (low_buffer_read TUInt8 TUInt128 h1 tag_b 0) == tag
+      ))))
+    )
 
 
 inline_for_extraction
